lib/lemmata_lean.ml
@@ -338,11 +338,8 @@ let rec resource_to_itp (global : Global.t) (t : CI.itp_resource_term) =
   | CI.ITP_PName (CI.ITP_sym nm, CI.ITP_sym pname, iargs, ptr) ->
     let args = List.map aux iargs in
     build ((Sym.pp pname :: aux ptr :: args) @ [ Sym.pp nm ])
-  | CI.ITP_Each _ ->
-    rets "Each is unsupported in Lean right now"
-    (* TODO: pending upstream decisions about arrays *)
   | CI.ITP_Good -> rets ""
-  | CI.ITP_scalar _ | CI.ITP_block_sized _ ->
+  | CI.ITP_scalar _ | CI.ITP_owned_value _ | CI.ITP_block_sized _ | CI.ITP_each_resource _ ->
     failwith "Typed memory resources are currently supported only by the Rocq exporter"
   | CI.ITP_Unsupported_Resource msg -> rets msg
 
