tests/rocq_lemmas/proofs/memory/IteratedInteger_Proof.v
@@ -1,0 +1,37 @@
+From Stdlib Require Import ZArith.
+From iris.proofmode Require Import proofmode.
+From iris.base_logic Require Import invariants.
+Require Import IteratedExport.IteratedInteger.
+
+Module Inst <: Parameters.
+End Inst.
+
+Module InstOK <: Lemma_Spec(Inst).
+  Module L := Lemma_Defs(Inst).
+  Import L L.D L.R.
+  Open Scope Z_scope.
+
+  Section Proof.
+    Context {cn_selectors : Selectors} `{!heapGS_gen Σ}.
+    Local Notation "⊢ P" := (⊢@{iPropI Σ} P).
+
+    Lemma each_w_negative_sparse : ⊢ each_w_negative_sparse_type.
+    Proof.
+      iIntros (p) "H %Halign". iExists tt. iSplitL; last done.
+      rewrite NegativeSparseW_unfold. iSplit; first done. iFrame. done.
+    Qed.
+
+    Lemma each_w_integer_identity : ⊢ each_w_integer_identity_type.
+    Proof. iIntros (p n) "H %Halign". iFrame. done. Qed.
+
+    Lemma each_rw_signed_map : ⊢ each_rw_signed_map_type.
+    Proof.
+      iIntros (p before) "H %Halign Hrepresentable %Hvalue".
+      iExists before. iFrame. done.
+    Qed.
+  End Proof.
+End InstOK.
+
+Print Assumptions InstOK.each_w_negative_sparse.
+Print Assumptions InstOK.each_w_integer_identity.
+Print Assumptions InstOK.each_rw_signed_map.
