tests/rocq_lemmas/proofs/memory/Iterated_Proof.v
@@ -1,0 +1,52 @@
+From Stdlib Require Import ZArith.
+From iris.proofmode Require Import proofmode.
+From iris.base_logic Require Import invariants.
+Require Import IteratedExport.Iterated.
+
+Module Inst <: Parameters.
+End Inst.
+
+Module InstOK <: Lemma_Spec(Inst).
+  Module L := Lemma_Defs(Inst).
+  Import L L.D L.R.
+  Open Scope Z_scope.
+
+  Section Proof.
+    Context {cn_selectors : Selectors} `{!heapGS_gen Σ}.
+    Local Notation "⊢ P" := (⊢@{iPropI Σ} P).
+
+    Lemma each_w_identity : ⊢ each_w_identity_type.
+    Proof. iIntros (p n) "H %Halign". iFrame. done. Qed.
+
+    Lemma each_w_sparse_identity : ⊢ each_w_sparse_identity_type.
+    Proof.
+      iIntros (p) "H %Halign". iExists tt. iSplitL; last done.
+      rewrite SparseW_unfold. iSplit; first done. iFrame. done.
+    Qed.
+
+    Lemma each_w_sparse_unpack : ⊢ each_w_sparse_unpack_type.
+    Proof.
+      iIntros (p before) "H". rewrite SparseW_unfold.
+      iDestruct "H" as "[_ [H [%Halign _]]]". iFrame. done.
+    Qed.
+
+    Lemma each_w_empty_has_id : ⊢ each_w_empty_has_id_type.
+    Proof.
+      iIntros (p) "[%Hid _] _". iSplitL; last done. iPureIntro.
+      destruct p as [[aid addr]|]; simpl in Hid; last contradiction.
+      unfold is_null, Memory.ptr_eq, Memory.null. simpl. tauto.
+    Qed.
+
+    Lemma each_rw_map_identity : ⊢ each_rw_map_identity_type.
+    Proof.
+      iIntros (p before) "H %Halign %Hvalue".
+      iExists before. iFrame. done.
+    Qed.
+  End Proof.
+End InstOK.
+
+Print Assumptions InstOK.each_w_identity.
+Print Assumptions InstOK.each_w_sparse_identity.
+Print Assumptions InstOK.each_w_sparse_unpack.
+Print Assumptions InstOK.each_w_empty_has_id.
+Print Assumptions InstOK.each_rw_map_identity.
