tests/rocq_lemmas/unit/memory/Iterated_Resource_Tests.v
@@ -1,0 +1,113 @@
+From Stdlib Require Import ZArith Lia.
+From stdpp Require Import infinite.
+From iris.proofmode Require Import proofmode.
+Require Import CN_Lemmas.CN_Memory_Iris.
+Open Scope Z_scope.
+
+Module IntegerVIP64 <: CONFIG.
+  Definition pointer_bits : nat := 64%nat.
+  Definition bitvectors := false.
+  Definition vip := true.
+End IntegerVIP64.
+Module M := CN_Memory_Iris.Make IntegerVIP64.
+Import M M.Memory.
+
+Section Iteration.
+  Context {Σ : gFunctors}.
+
+  Lemma each_set (indices : gset Z) (body : Z -> iProp Σ) :
+    each_resource (fun i => i ∈ indices) body ⊣⊢
+      ([∗ set] i ∈ indices, body i).
+  Proof.
+    iSplit.
+    - iIntros "H". iDestruct "H" as (actual) "[%Hactual H]".
+      assert (actual = indices) as -> by (apply set_eq; exact Hactual).
+      iExact "H".
+    - iIntros "H". iExists indices. iFrame. done.
+  Qed.
+
+  Lemma each_guard_equiv (selected selected' : Z -> Prop) (body : Z -> iProp Σ) :
+    (forall i, selected i <-> selected' i) ->
+    each_resource selected body ⊣⊢ each_resource selected' body.
+  Proof.
+    intros Heq. iSplit; iIntros "H";
+      iDestruct "H" as (indices) "[%Hindices H]";
+      iExists indices; iFrame; iPureIntro; intro i;
+      specialize (Hindices i); specialize (Heq i); tauto.
+  Qed.
+
+  Lemma each_empty (body : Z -> iProp Σ) :
+    each_resource (fun _ => False%type) body ⊣⊢ emp.
+  Proof.
+    rewrite (each_guard_equiv _ (fun i => i ∈ (∅ : gset Z)) body);
+      last (intro i; set_solver).
+    rewrite each_set big_sepS_empty. done.
+  Qed.
+
+  Lemma each_singleton (index : Z) (body : Z -> iProp Σ) :
+    each_resource (fun i => i = index) body ⊣⊢ body index.
+  Proof.
+    rewrite (each_guard_equiv _ (fun i => i ∈ ({[index]} : gset Z)) body);
+      last (intro i; set_solver).
+    rewrite each_set big_sepS_singleton. done.
+  Qed.
+
+  Lemma each_disjoint_union (left right : gset Z) (body : Z -> iProp Σ) :
+    left ## right ->
+    each_resource (fun i => i ∈ left ∪ right) body ⊣⊢
+      each_resource (fun i => i ∈ left) body ∗
+      each_resource (fun i => i ∈ right) body.
+  Proof. intros Hdisjoint. rewrite !each_set big_sepS_union //. Qed.
+
+  Lemma each_sparse_negative (body : Z -> iProp Σ) :
+    each_resource (fun i => i = -7 \/ i = 11) body ⊣⊢ body (-7) ∗ body 11.
+  Proof.
+    rewrite (each_guard_equiv _ (fun i => i ∈ ({[-7]} ∪ {[11]} : gset Z)) body);
+      last (intro i; set_solver).
+    rewrite each_disjoint_union; last set_solver.
+    rewrite !each_set !big_sepS_singleton. done.
+  Qed.
+
+  Lemma each_sparse_permutation (body : Z -> iProp Σ) :
+    each_resource (fun i => i = -7 \/ i = 11) body ⊣⊢
+      each_resource (fun i => i = 11 \/ i = -7) body.
+  Proof. apply each_guard_equiv. intros; tauto. Qed.
+
+  (* A finite support is not conjured for an arbitrary infinite guard. *)
+  Lemma each_infinite_impossible (body : Z -> iProp Σ) :
+    each_resource (fun _ => True%type) body ⊢ False.
+  Proof.
+    iIntros "H". iDestruct "H" as (indices) "[%Hindices _]".
+    iPureIntro.
+    pose proof (is_fresh indices) as Hfresh.
+    apply Hfresh. apply Hindices. done.
+  Qed.
+End Iteration.
+
+Section ExclusiveOwnership.
+  Context `{!M.heapGS_gen Σ}.
+
+  Definition one_byte (location : Address) (value : Val) : iProp Σ :=
+    @pointsto Address address_eq_dec address_countable Val Σ heapGS_gen_heapGS
+      location (DfracOwn 1) value.
+
+  (* Different iteration indices do not permit aliasing full byte ownership. *)
+  Lemma each_aliasing_byte_impossible (location : Address) (value : Val) :
+    each_resource (fun i => i = -7 \/ i = 11)
+      (fun _ => one_byte location value) ⊢ False.
+  Proof.
+    rewrite each_sparse_negative. iIntros "[Hleft Hright]".
+    iDestruct (pointsto_ne with "Hleft Hright") as %Hinvalid.
+    done.
+  Qed.
+End ExclusiveOwnership.
+
+Print Assumptions each_set.
+Print Assumptions each_guard_equiv.
+Print Assumptions each_empty.
+Print Assumptions each_singleton.
+Print Assumptions each_disjoint_union.
+Print Assumptions each_sparse_negative.
+Print Assumptions each_sparse_permutation.
+Print Assumptions each_infinite_impossible.
+Print Assumptions each_aliasing_byte_impossible.
